\documentclass{article}
\usepackage{xeCJK}
\usepackage{amsmath}
\usepackage{amssymb}
\usepackage{mathrsfs}
\usepackage{bm}
\usepackage{hyperref}
\usepackage{graphicx}
\usepackage{subcaption}
\usepackage{float}
\usepackage{multicol}
\usepackage[ruled,linesnumbered]{algorithm2e}

\setlength{\parindent}{2em}
\usepackage{geometry}
\geometry{a4paper, left=2.54cm, right=2.54cm, top=3.18cm, bottom=3.18cm}

% 设置文章行距
\renewcommand{\baselinestretch}{1.5}

% 定义引用格式
% \newcommand{\myeqref}[1]{\eqref{#1}式}
% \newcommand{\figref}[1]{图\ref{#1}}
% \newcommand{\tabref}[1]{表\ref{#1}}
\title{\textbf{Two Coupled Oscillators with Chirality}}

\begin{document}

\maketitle

\section{The Model}

\subsection{Raw model}

$$
\begin{cases}
	\dot{x}_{1,2}=v\cos \theta _{1,2}\\
	\dot{y}_{1,2}=v\sin \theta _{1,2}\\
	\dot{\theta}_{1,2}=\omega _{1,2}+\lambda f\left( r \right) \sin \left( \theta _{2,1}-\theta _{1,2} \right)\\
\end{cases}
$$
where $f\left( r \right)$ is a function of $r=\left| \mathbf{r}_1-\mathbf{r}_2 \right|$, and $\lambda$ is the coupling strength. The function $f\left( r \right)$ can be defined as

\begin{enumerate}
    \item $f\left( r \right) _H=H\left( r_0-r \right),\;r_0>0$;
    \item $f\left( r \right) _P=\left( 1+\frac{r}{r_0} \right) ^{-\frac{1}{r_0}},\;r_0>0$;
    \item $\dots$
\end{enumerate}

\subsection{Model under polar coordinates}

Let
$$
\begin{aligned}
	x_i&=r_i\cos \varphi _i\;,\\
	y_i&=r_i\sin \varphi _i\;,\\
\end{aligned}
$$
then we have
$$
\begin{aligned}
	\dot{r}_i&=\frac{1}{r_i}\left( x_i\dot{x}_i+y_i\dot{y}_i \right)\\
	&=v\cos \varphi _i\cos \theta _i+v\sin \varphi _i\sin \theta _i\\
	&=v\cos \left( \varphi _i-\theta _i \right)\;,\\
	\dot{\varphi}_i&=\frac{1}{r_{i}^{2}}\left( x\dot{y}-y\dot{x} \right)\\
	&=\frac{v}{r_i}\left( \sin \varphi _i\cos \theta _i-\cos \varphi _i\sin \theta _i \right)\\
	&=\frac{v}{r_i}\sin \left( \varphi _i-\theta _i \right)\;.\\
\end{aligned}
$$
Introduce $\alpha_i=\varphi_i-\theta_i$, $\Delta \theta =\theta _2-\theta _1$, $\Delta \varphi =\varphi _2-\varphi _1$, $\Delta \omega =\omega _2-\omega _1$, then we have

\begin{equation}\label{eq:l1.2}
    \begin{cases}
        \dot{r}_{1,2}=v\cos \alpha _{1,2}\\
        \dot{\alpha}_{1,2}=\frac{v}{r_{1,2}}\sin \alpha _{1,2}-\omega _{1,2}\mp \lambda f\left( r \right) \sin \Delta \theta\\
        \Delta \dot{\varphi}=\frac{v}{r_2}\sin \alpha _2-\frac{v}{r_1}\sin \alpha _1\\
        \Delta \dot{\theta}=\Delta \omega -2\lambda f\left( r \right) \sin \Delta \theta\\
    \end{cases}
\end{equation}
where
$$
\begin{aligned}
	r&=\sqrt{\left( r_1\cos \varphi _1-r_2\cos \varphi _2 \right) ^2+\left( r_1\sin \varphi _1-r_2\sin \varphi _2 \right) ^2}\\
	&=\sqrt{r_{1}^{2}+r_{2}^{2}-2r_1r_2\cos \Delta \varphi}\\
\end{aligned}\;.
$$
So the function $f\left( r \right)$ can be defined as $f\left( r_1,r_2,\Delta \varphi \right)$.

\subsection{Single direction driving}

Assuming that $\dot{\theta}_2=\omega _2, \alpha_2=\cfrac{\pi\text{sgn}\omega_2}{2}$, which means that the second oscillator is rotating around the origin with a constant angular velocity $\omega_2$, and the first oscillator is driven by the second one. Then the model becomes
$$
\begin{cases}
    \dot{r}_1=v\cos \alpha _1\\
    \dot{\alpha}_1=\frac{v}{r_1}\sin \alpha _1-\omega _1-\lambda f\left( r \right) \sin \Delta \theta\\
    \Delta \dot{\varphi}=\omega _2-\frac{v}{r_1}\sin \alpha _1\\
    \Delta \dot{\theta}=\Delta \omega -\lambda f\left( r \right) \sin \Delta \theta\\
\end{cases}\;.
$$
When $2\lambda f\left( r \right) \geqslant \left| \Delta \omega \right|$, the system has fixed points $\mathbf{x}$, which are
$$
\begin{aligned}
	r_1&=\frac{v}{\omega _2}\;,\\
	\alpha _1&=\frac{\pi \text{sgn} \omega _2}{2}\;,\\
	\Delta \varphi &=C_{\varphi}\;,\\
	\Delta \theta &=C_{\theta}\;,\\
\end{aligned}
$$
where $C_{\varphi}$ and $C_{\theta}$ are constants determined by the initial conditions. Linearizing the governing equations yields
$$
M=\left[ \begin{matrix}
	0&		-v\sin \alpha _1&		0&		0\\
	-\frac{v}{r_{1}^{2}}\sin \alpha _1-\lambda f_{r_1}\sin \Delta \theta&		\frac{v}{r_1}\cos \alpha _1&		-\lambda f_{\Delta \varphi}\sin \Delta \theta&		-\lambda f\cos \Delta \theta\\
	\frac{v}{r_{1}^{2}}\sin \alpha _1&		-\frac{v}{r_1}\cos \alpha _1&		0&		0\\
	-\lambda f_{r_1}\sin \Delta \theta&		0&		-\lambda f_{\Delta \varphi}\sin \Delta \theta&		-\lambda f\cos \Delta \theta\\
\end{matrix} \right] 
$$
where $f_{r_1}=\cfrac{\partial f}{\partial r_1}$, $f_{\Delta \varphi}=\cfrac{\partial f}{\partial \Delta \varphi}$, and $f_{\Delta \theta}=\cfrac{\partial f}{\partial \Delta \theta}$. Evaluating $M$ at the fixed points results in
$$
M=\left[ \begin{matrix}
	0&		-v\text{sgn} \omega _2&		0&		0\\
	-\frac{\omega _{2}^{2}}{v}\text{sgn} \omega _2-\lambda f_{r_1}\left( \mathbf{x} \right) \sin C_{\theta}&		0&		-\lambda f_{\Delta \varphi}\left( \mathbf{x} \right) \sin C_{\theta}&		-\lambda f\left( \mathbf{x} \right) \cos C_{\theta}\\
	\frac{\omega _{2}^{2}}{v}\text{sgn} \omega _2&		0&		0&		0\\
	-\lambda f_{r_1}\left( \mathbf{x} \right) \sin C_{\theta}&		0&		-\lambda f_{\Delta \varphi}\left( \mathbf{x} \right) \sin C_{\theta}&		-\lambda f\left( \mathbf{x} \right) \cos C_{\theta}\\
\end{matrix} \right] 
$$


\end{document}